Leanbin/Init/Data/Char/Lemmas.lean
@@ -6,24 +6,24 @@ import Leanbin.Init.Data.Char.Basic
 
 namespace Char
 
-theorem val_of_nat_eq_of_is_valid {n : Nat} : IsValidChar n → (ofNat n).val = n := by
+theorem val_ofNat_eq_of_is_valid {n : Nat} : IsValidChar n → (ofNat n).val = n := by
   intro h <;> unfold of_nat <;> rw [dif_pos h]
-#align char.val_of_nat_eq_of_is_valid Char.val_of_nat_eq_of_is_valid
+#align char.val_of_nat_eq_of_is_valid Char.val_ofNat_eq_of_is_valid
 
-theorem val_of_nat_eq_of_not_is_valid {n : Nat} : ¬IsValidChar n → (ofNat n).val = 0 := by
+theorem val_ofNat_eq_of_not_is_valid {n : Nat} : ¬IsValidChar n → (ofNat n).val = 0 := by
   intro h <;> unfold of_nat <;> rw [dif_neg h]
-#align char.val_of_nat_eq_of_not_is_valid Char.val_of_nat_eq_of_not_is_valid
+#align char.val_of_nat_eq_of_not_is_valid Char.val_ofNat_eq_of_not_is_valid
 
-theorem of_nat_eq_of_not_is_valid {n : Nat} : ¬IsValidChar n → ofNat n = ofNat 0 := by
+theorem ofNat_eq_of_not_is_valid {n : Nat} : ¬IsValidChar n → ofNat n = ofNat 0 := by
   intro h <;> apply eq_of_veq <;> rw [val_of_nat_eq_of_not_is_valid h] <;> rfl
-#align char.of_nat_eq_of_not_is_valid Char.of_nat_eq_of_not_is_valid
+#align char.of_nat_eq_of_not_is_valid Char.ofNat_eq_of_not_is_valid
 
-theorem of_nat_ne_of_ne {n₁ n₂ : Nat} (h₁ : n₁ ≠ n₂) (h₂ : IsValidChar n₁) (h₃ : IsValidChar n₂) :
+theorem ofNat_ne_of_ne {n₁ n₂ : Nat} (h₁ : n₁ ≠ n₂) (h₂ : IsValidChar n₁) (h₃ : IsValidChar n₂) :
     ofNat n₁ ≠ ofNat n₂ := by
   apply ne_of_vne
   rw [val_of_nat_eq_of_is_valid h₂, val_of_nat_eq_of_is_valid h₃]
   assumption
-#align char.of_nat_ne_of_ne Char.of_nat_ne_of_ne
+#align char.of_nat_ne_of_ne Char.ofNat_ne_of_ne
 
 end Char
 
