Leanbin/Init/Data/Int/CompLemmas.lean
@@ -83,84 +83,90 @@ protected theorem nonneg_of_pos {a : ℤ} : 0 < a → 0 ≤ a :=
 /-! 3. nat_abs auxiliary lemmas -/
 
 
-theorem neg_succ_of_nat_lt_zero (n : ℕ) : negSucc n < 0 :=
+/- warning: int.neg_succ_of_nat_lt_zero clashes with int.neg_succ_lt_zero -> Int.negSucc_lt_zero
+Case conversion may be inaccurate. Consider using '#align int.neg_succ_of_nat_lt_zero Int.negSucc_lt_zeroₓ'. -/
+#print Int.negSucc_lt_zero /-
+theorem negSucc_lt_zero (n : ℕ) : negSucc n < 0 :=
   @lt.intro _ _ n
     (by
       simp [neg_succ_of_nat_coe, Int.ofNat_succ, Int.ofNat_add, Int.ofNat_one, Int.add_comm,
         Int.add_left_comm, Int.neg_add, Int.add_right_neg, Int.zero_add])
-#align int.neg_succ_of_nat_lt_zero Int.neg_succ_of_nat_lt_zero
+#align int.neg_succ_of_nat_lt_zero Int.negSucc_lt_zero
+-/
 
-theorem zero_le_of_nat (n : ℕ) : 0 ≤ ofNat n :=
+theorem zero_le_ofNat (n : ℕ) : 0 ≤ ofNat n :=
   @le.intro _ _ n (by rw [Int.zero_add, Int.coe_nat_eq])
-#align int.zero_le_of_nat Int.zero_le_of_nat
+#align int.zero_le_of_nat Int.zero_le_ofNat
 
-theorem of_nat_nat_abs_eq_of_nonneg : ∀ {a : ℤ}, 0 ≤ a → ofNat (natAbs a) = a
+#print Int.ofNat_natAbs_eq_of_nonneg /-
+theorem ofNat_natAbs_eq_of_nonneg : ∀ {a : ℤ}, 0 ≤ a → ofNat (natAbs a) = a
   | of_nat n, h => rfl
-  | neg_succ_of_nat n, h => absurd (neg_succ_of_nat_lt_zero n) (not_lt_of_ge h)
-#align int.of_nat_nat_abs_eq_of_nonneg Int.of_nat_nat_abs_eq_of_nonneg
+  | neg_succ_of_nat n, h => absurd (negSucc_lt_zero n) (not_lt_of_ge h)
+#align int.of_nat_nat_abs_eq_of_nonneg Int.ofNat_natAbs_eq_of_nonneg
+-/
 
-theorem ne_of_nat_abs_ne_nat_abs_of_nonneg {a b : ℤ} (ha : 0 ≤ a) (hb : 0 ≤ b)
+theorem ne_of_natAbs_ne_natAbs_of_nonneg {a b : ℤ} (ha : 0 ≤ a) (hb : 0 ≤ b)
     (h : natAbs a ≠ natAbs b) : a ≠ b := fun h =>
   by
   have : ofNat (natAbs a) = ofNat (natAbs b) := by
     rwa [of_nat_nat_abs_eq_of_nonneg ha, of_nat_nat_abs_eq_of_nonneg hb]
   injection this
   contradiction
-#align int.ne_of_nat_abs_ne_nat_abs_of_nonneg Int.ne_of_nat_abs_ne_nat_abs_of_nonneg
+#align int.ne_of_nat_abs_ne_nat_abs_of_nonneg Int.ne_of_natAbs_ne_natAbs_of_nonneg
 
 protected theorem ne_of_nat_ne_nonneg_case {a b : ℤ} {n m : Nat} (ha : 0 ≤ a) (hb : 0 ≤ b)
     (e1 : natAbs a = n) (e2 : natAbs b = m) (h : n ≠ m) : a ≠ b :=
   have : natAbs a ≠ natAbs b := by rwa [e1, e2]
-  ne_of_nat_abs_ne_nat_abs_of_nonneg ha hb this
+  ne_of_natAbs_ne_natAbs_of_nonneg ha hb this
 #align int.ne_of_nat_ne_nonneg_case Int.ne_of_nat_ne_nonneg_case
 
 /-! 4. Aux lemmas for pushing nat_abs inside numerals
    nat_abs_zero and nat_abs_one are defined at init/data/int/basic.lean -/
 
 
-theorem nat_abs_of_nat_core (n : ℕ) : natAbs (ofNat n) = n :=
+theorem natAbs_ofNat_core (n : ℕ) : natAbs (ofNat n) = n :=
   rfl
-#align int.nat_abs_of_nat_core Int.nat_abs_of_nat_core
+#align int.nat_abs_of_nat_core Int.natAbs_ofNat_core
 
-theorem nat_abs_of_neg_succ_of_nat (n : ℕ) : natAbs (negSucc n) = Nat.succ n :=
+theorem natAbs_of_negSucc (n : ℕ) : natAbs (negSucc n) = Nat.succ n :=
   rfl
-#align int.nat_abs_of_neg_succ_of_nat Int.nat_abs_of_neg_succ_of_nat
+#align int.nat_abs_of_neg_succ_of_nat Int.natAbs_of_negSucc
 
-protected theorem nat_abs_add_nonneg :
+protected theorem natAbs_add_nonneg :
     ∀ {a b : Int}, 0 ≤ a → 0 ≤ b → natAbs (a + b) = natAbs a + natAbs b
   | of_nat n, of_nat m, h₁, h₂ =>
     by
     have : ofNat n + ofNat m = ofNat (n + m) := rfl
     simp [nat_abs_of_nat_core, this]
-  | _, neg_succ_of_nat m, h₁, h₂ => absurd (neg_succ_of_nat_lt_zero m) (not_lt_of_ge h₂)
-  | neg_succ_of_nat n, _, h₁, h₂ => absurd (neg_succ_of_nat_lt_zero n) (not_lt_of_ge h₁)
-#align int.nat_abs_add_nonneg Int.nat_abs_add_nonneg
+  | _, neg_succ_of_nat m, h₁, h₂ => absurd (negSucc_lt_zero m) (not_lt_of_ge h₂)
+  | neg_succ_of_nat n, _, h₁, h₂ => absurd (negSucc_lt_zero n) (not_lt_of_ge h₁)
+#align int.nat_abs_add_nonneg Int.natAbs_add_nonneg
 
-protected theorem nat_abs_add_neg :
+protected theorem natAbs_add_neg :
     ∀ {a b : Int}, a < 0 → b < 0 → natAbs (a + b) = natAbs a + natAbs b
   | neg_succ_of_nat n, neg_succ_of_nat m, h₁, h₂ =>
     by
     have : -[n+1] + -[m+1] = -[Nat.succ (n + m)+1] := rfl
     simp [nat_abs_of_neg_succ_of_nat, this, Nat.succ_add, Nat.add_succ]
-#align int.nat_abs_add_neg Int.nat_abs_add_neg
+#align int.nat_abs_add_neg Int.natAbs_add_neg
 
-protected theorem nat_abs_bit0 : ∀ a : Int, natAbs (bit0 a) = bit0 (natAbs a)
-  | of_nat n => Int.nat_abs_add_nonneg (zero_le_of_nat n) (zero_le_of_nat n)
-  | neg_succ_of_nat n => Int.nat_abs_add_neg (neg_succ_of_nat_lt_zero n) (neg_succ_of_nat_lt_zero n)
-#align int.nat_abs_bit0 Int.nat_abs_bit0
+protected theorem natAbs_bit0 : ∀ a : Int, natAbs (bit0 a) = bit0 (natAbs a)
+  | of_nat n => Int.natAbs_add_nonneg (zero_le_ofNat n) (zero_le_ofNat n)
+  | neg_succ_of_nat n => Int.natAbs_add_neg (negSucc_lt_zero n) (negSucc_lt_zero n)
+#align int.nat_abs_bit0 Int.natAbs_bit0
 
-protected theorem nat_abs_bit0_step {a : Int} {n : Nat} (h : natAbs a = n) :
-    natAbs (bit0 a) = bit0 n := by rw [← h]; apply Int.nat_abs_bit0
-#align int.nat_abs_bit0_step Int.nat_abs_bit0_step
+protected theorem natAbs_bit0_step {a : Int} {n : Nat} (h : natAbs a = n) :
+    natAbs (bit0 a) = bit0 n := by rw [← h]; apply Int.natAbs_bit0
+#align int.nat_abs_bit0_step Int.natAbs_bit0_step
 
-protected theorem nat_abs_bit1_nonneg {a : Int} (h : 0 ≤ a) : natAbs (bit1 a) = bit1 (natAbs a) :=
+protected theorem natAbs_bit1_nonneg {a : Int} (h : 0 ≤ a) : natAbs (bit1 a) = bit1 (natAbs a) :=
   show natAbs (bit0 a + 1) = bit0 (natAbs a) + natAbs 1 by
-    rw [Int.nat_abs_add_nonneg (Int.bit0_nonneg h) (le_of_lt Int.zero_lt_one), Int.nat_abs_bit0]
-#align int.nat_abs_bit1_nonneg Int.nat_abs_bit1_nonneg
+    rw [Int.natAbs_add_nonneg (Int.bit0_nonneg h) (le_of_lt Int.zero_lt_one), Int.natAbs_bit0]
+#align int.nat_abs_bit1_nonneg Int.natAbs_bit1_nonneg
 
-protected theorem nat_abs_bit1_nonneg_step {a : Int} {n : Nat} (h₁ : 0 ≤ a) (h₂ : natAbs a = n) :
-    natAbs (bit1 a) = bit1 n := by rw [← h₂]; apply Int.nat_abs_bit1_nonneg h₁
-#align int.nat_abs_bit1_nonneg_step Int.nat_abs_bit1_nonneg_step
+protected theorem natAbs_bit1_nonneg_step {a : Int} {n : Nat} (h₁ : 0 ≤ a) (h₂ : natAbs a = n) :
+    natAbs (bit1 a) = bit1 n := by rw [← h₂]; apply Int.natAbs_bit1_nonneg h₁
+#align int.nat_abs_bit1_nonneg_step Int.natAbs_bit1_nonneg_step
 
 end Int
 
