Leanbin/Init/Data/String/Ops.lean
@@ -18,23 +18,23 @@ namespace String
 namespace Iterator
 
 @[simp]
-theorem next_to_string_mk_iterator (s : String) : s.mkIterator.nextToString = s := by
+theorem nextToString_mkIterator (s : String) : s.mkIterator.nextToString = s := by
   induction s <;> rfl
-#align string.iterator.next_to_string_mk_iterator String.Iterator.next_to_string_mk_iterator
+#align string.iterator.next_to_string_mk_iterator String.Iterator.nextToString_mkIterator
 
 @[simp]
-theorem length_next_to_string_next (it : Iterator) :
+theorem length_nextToString_next (it : Iterator) :
     it.next.nextToString.length = it.nextToString.length - 1 := by
   cases it <;> cases it_snd <;>
     simp [iterator.next, iterator.next_to_string, String.length, Nat.add_sub_cancel_left]
-#align string.iterator.length_next_to_string_next String.Iterator.length_next_to_string_next
+#align string.iterator.length_next_to_string_next String.Iterator.length_nextToString_next
 
-theorem zero_lt_length_next_to_string_of_has_next {it : Iterator} :
+theorem zero_lt_length_nextToString_of_hasNext {it : Iterator} :
     it.hasNext → 0 < it.nextToString.length := by
   cases it <;> cases it_snd <;>
     simp [iterator.has_next, iterator.next_to_string, String.length, Nat.zero_lt_one_add,
       Nat.add_comm, false_imp_iff]
-#align string.iterator.zero_lt_length_next_to_string_of_has_next String.Iterator.zero_lt_length_next_to_string_of_has_next
+#align string.iterator.zero_lt_length_next_to_string_of_has_next String.Iterator.zero_lt_length_nextToString_of_hasNext
 
 end Iterator
 
@@ -45,7 +45,7 @@ private def split_core (p : Char → Bool) : Iterator → Iterator → List Stri
     if h : stop.hasNext then
       -- wf hint
       have : stop.nextToString.length - 1 < stop.nextToString.length :=
-        Nat.sub_lt (Iterator.zero_lt_length_next_to_string_of_has_next h) (by decide)
+        Nat.sub_lt (Iterator.zero_lt_length_nextToString_of_hasNext h) (by decide)
       if p stop.curr then
         let rest := stop.next.nextToString
         (start.extract stop).getOrElse "" :: split_core stop.next stop.next
