Leanbin/Init/Meta/Name.lean
@@ -30,9 +30,9 @@ def autoParam.{u} (α : Sort u) (tac_name : Name) : Sort u :=
 #align auto_param autoParamₓ
 
 @[simp]
-theorem auto_param_eq.{u} (α : Sort u) (n : Name) : autoParam α n = α :=
+theorem autoParam_eq.{u} (α : Sort u) (n : Name) : autoParam α n = α :=
   rfl
-#align auto_param_eq auto_param_eq
+#align auto_param_eq autoParamₓ_eq
 
 instance : Inhabited Name :=
   ⟨Name.anonymous⟩
